midstream

examples/algorithms/gc.fst
@@ -1,3 +1,7 @@
+(*--build-config
+    options:--max_ifuel 1 --initial_ifuel 1 --max_fuel 1 --initial_fuel 1;
+    other-files:
+  --*)
 module GC
 
 (* invariants *)
@@ -46,30 +50,34 @@ type gc_state = {
   fields: field_map
 }
 
+opaque type ptr_lifts gc_state (ptr:mem_addr) : Type =
+  b2t (valid (gc_state.to_abs ptr))
+
 opaque type ptr_lifts_to gc_state (ptr:mem_addr) (abs:abs_node) : Type =
   valid abs
   /\ gc_state.to_abs ptr = abs
 
 opaque type obj_inv gc_state (i:mem_addr) =
   valid (gc_state.to_abs i)
-  ==> ptr_lifts_to gc_state (gc_state.fields i F1) (gc_state.abs_fields (gc_state.to_abs i) F1)
-   /\ ptr_lifts_to gc_state (gc_state.fields i F2) (gc_state.abs_fields (gc_state.to_abs i) F2)
+  ==> (ptr_lifts_to gc_state (gc_state.fields i F1) (gc_state.abs_fields (gc_state.to_abs i) F1)
+   /\  ptr_lifts_to gc_state (gc_state.fields i F2) (gc_state.abs_fields (gc_state.to_abs i) F2))
 
 (* Maybe derive gc_inv from mutator_inv? via some higher-orderness *)
 opaque type gc_inv gc_state =
   to_abs_inj gc_state.to_abs
   /\ (forall (i:mem_addr).
         obj_inv gc_state i
-        /\ (gc_state.color i = Black ==> gc_state.color (gc_state.fields i F1) <> White
-                                     /\ gc_state.color (gc_state.fields i F2) <> White)
-        /\ not (valid (gc_state.to_abs i)) <==> gc_state.color i = Unalloc)
+        /\ (gc_state.color i = Black ==> (gc_state.color (gc_state.fields i F1) <> White
+                                       /\ gc_state.color (gc_state.fields i F2) <> White))
+        /\ (not (valid (gc_state.to_abs i)) <==> gc_state.color i = Unalloc))
 
+opaque logic type trigger (i:int) = True
 opaque type mutator_inv gc_state =
   to_abs_inj gc_state.to_abs
-  /\ (forall (i:mem_addr).
-        obj_inv gc_state i
-        /\ (gc_state.color i = Unalloc \/ gc_state.color i = White)
-        /\ not (valid (gc_state.to_abs i)) <==> gc_state.color i = Unalloc)
+  /\ (forall (i:mem_addr).{:pattern (trigger i)}
+        obj_inv gc_state i /\
+        (gc_state.color i = Unalloc \/ gc_state.color i = White) /\
+        (not (valid (gc_state.to_abs i)) <==> gc_state.color i = Unalloc))
 
 new_effect GC_STATE = STATE_h gc_state
 kind GCPost (a:Type) = a -> gc_state -> Type
@@ -98,19 +106,95 @@ type init_invariant (ptr:mem_addr) (gc:gc_state) =
 val upd_map: #a:Type -> #b:Type -> (a -> Tot b) -> a -> b -> a -> Tot b
 let upd_map f i v = fun j -> if i=j then v else f j
 
-val aux : ptr:mem_addr -> GC unit
+val aux_init : ptr:mem_addr -> GC unit
                             (requires (init_invariant ptr))
                             (ensures (fun gc _ gc' -> mutator_inv gc'))
-let rec aux ptr =
+let rec aux_init ptr =
   let gc = get () in
   let gc' = {gc with
       color=upd_map gc.color ptr Unalloc;
       to_abs=upd_map gc.to_abs ptr no_abs
     } in
   set gc';
-  if ptr + 1 < mem_hi then aux (ptr + 1)
+  if ptr + 1 < mem_hi then aux_init (ptr + 1)
 
 val initialize: unit -> GC unit
     (requires (fun g -> True))
-    (ensures (fun g _ g' -> mutator_inv g' /\ to_abs_inj g'.to_abs))
-let initialize () = aux mem_lo  (* TODO: hoisting aux is super ugly ... fix! *)
+    (ensures (fun g _ g' -> mutator_inv g'))
+let initialize () = aux_init mem_lo  (* TODO: hoisting aux is super ugly ... fix! *)
+
+val read_field : ptr:mem_addr -> f:field -> GCMut mem_addr
+  (requires (fun gc -> ptr_lifts_to gc ptr (gc.to_abs ptr)))
+  (ensures (fun gc i gc' -> gc=gc'
+            /\ ptr_lifts_to gc' i (gc.abs_fields (gc.to_abs ptr) f)))
+let read_field ptr f =
+  cut (trigger ptr);
+  let gc = get () in
+  gc.fields ptr f
+
+val upd_field: field_map
+            -> mem_addr
+            -> field
+            -> mem_addr
+            -> Tot field_map
+let upd_field m i f v =
+  fun j g -> if (i, f) = (j, g) then v else m j g
+
+val upd_abs_field: abs_field_map
+            -> abs_node
+            -> field
+            -> abs_node
+            -> Tot abs_field_map
+let upd_abs_field m i f v =
+  fun j g -> if (i, f) = (j, g) then v else m j g
+
+opaque type mutator_inv' gc_state =
+    to_abs_inj gc_state.to_abs
+    /\ (forall (i:mem_addr).//{:pattern (trigger i)}
+          obj_inv gc_state i /\
+          (gc_state.color i = Unalloc \/ gc_state.color i = White) /\
+          (not (valid (gc_state.to_abs i)) <==> gc_state.color i = Unalloc) /\
+          True
+          )
+module VerifyThis
+open GC
+(*val write_field: ptr:mem_addr -> f:field -> v:mem_addr -> GC unit
+  (requires (fun gc -> ptr_lifts gc ptr /\ ptr_lifts gc v /\ mutator_inv' gc))
+  (ensures (fun gc _ gc' ->
+              to_abs_inj gc'.to_abs
+                /\ obj_inv gc' ptr
+                /\ obj_inv gc' v /\
+                (*/\ mutator_inv gc' /\*)
+                (*/\ (forall (i:mem_addr).{:pattern (trigger i)}
+                      obj_inv gc' i /\
+                      (*(gc'.color i = Unalloc \/ gc'.color i = White) /\*)
+                      (*(not (valid (gc'.to_abs i)) <==> gc'.color i = Unalloc)*)
+                      True
+                      )) /\*)
+              gc'.color=gc.color /\
+              gc'.to_abs = gc.to_abs /\
+              gc'.abs_fields
+               = upd_map #(abs_node * field) #abs_node gc.abs_fields (gc.to_abs ptr, f) (gc.to_abs v)))*)
+val write_field: ptr:mem_addr -> f:field -> v:mem_addr -> GC unit
+ (requires (fun gc -> ptr_lifts gc ptr /\ ptr_lifts gc v /\ mutator_inv' gc))
+ (ensures (fun gc _ gc' -> True))
+let write_field ptr f v =
+  (*cut (trigger ptr);
+  cut (trigger v);*)
+  let gc = get () in
+  (*assert (obj_inv gc v);*)
+  let gc' = {gc with
+    (*color=upd_map gc.color ptr (gc.color ptr)*)
+    fields=upd_field gc.fields ptr f (gc.fields ptr f);
+    abs_fields=upd_abs_field gc.abs_fields (gc.to_abs ptr) f (gc.to_abs (gc.fields ptr f));//v)
+    } in
+  (*assert (valid (gc'.to_abs v));
+  assert (v<>ptr ==> gc'.abs_fields (gc'.to_abs v, f) = gc.abs_fields (gc.to_abs v, f));
+  assert (v<>ptr ==> gc'.fields (v, f) = gc.fields (v, f));
+  assert (ptr_lifts_to gc' (gc'.fields (v, f)) (gc'.abs_fields (gc'.to_abs v, f)));
+  assert (obj_inv gc' v);
+  assert (obj_inv gc' ptr);
+  assert (mutator_inv gc);*)
+  assert (mutator_inv' gc');
+  admit();
+  set gc'
